src/HOL/Enum.thy
@@ -491,9 +491,9 @@ end
 
 subsection {* Small finite types *}
 
-text {* We define small finite types for the use in Quickcheck *}
+text {* We define small finite types for use in Quickcheck *}
 
-datatype finite_1 = a\<^sub>1
+datatype (plugins only: code "quickcheck*") finite_1 = a\<^sub>1
 
 notation (output) a\<^sub>1  ("a\<^sub>1")
 
@@ -595,7 +595,7 @@ end
 declare [[simproc del: finite_1_eq]]
 hide_const (open) a\<^sub>1
 
-datatype finite_2 = a\<^sub>1 | a\<^sub>2
+datatype (plugins only: code "quickcheck*") finite_2 = a\<^sub>1 | a\<^sub>2
 
 notation (output) a\<^sub>1  ("a\<^sub>1")
 notation (output) a\<^sub>2  ("a\<^sub>2")
@@ -701,7 +701,7 @@ end
 
 hide_const (open) a\<^sub>1 a\<^sub>2
 
-datatype finite_3 = a\<^sub>1 | a\<^sub>2 | a\<^sub>3
+datatype (plugins only: code "quickcheck*") finite_3 = a\<^sub>1 | a\<^sub>2 | a\<^sub>3
 
 notation (output) a\<^sub>1  ("a\<^sub>1")
 notation (output) a\<^sub>2  ("a\<^sub>2")
@@ -825,7 +825,7 @@ end
 
 hide_const (open) a\<^sub>1 a\<^sub>2 a\<^sub>3
 
-datatype finite_4 = a\<^sub>1 | a\<^sub>2 | a\<^sub>3 | a\<^sub>4
+datatype (plugins only: code "quickcheck*") finite_4 = a\<^sub>1 | a\<^sub>2 | a\<^sub>3 | a\<^sub>4
 
 notation (output) a\<^sub>1  ("a\<^sub>1")
 notation (output) a\<^sub>2  ("a\<^sub>2")
@@ -926,8 +926,7 @@ end
 
 hide_const (open) a\<^sub>1 a\<^sub>2 a\<^sub>3 a\<^sub>4
 
-
-datatype finite_5 = a\<^sub>1 | a\<^sub>2 | a\<^sub>3 | a\<^sub>4 | a\<^sub>5
+datatype (plugins only: code "quickcheck*") finite_5 = a\<^sub>1 | a\<^sub>2 | a\<^sub>3 | a\<^sub>4 | a\<^sub>5
 
 notation (output) a\<^sub>1  ("a\<^sub>1")
 notation (output) a\<^sub>2  ("a\<^sub>2")
